simplify doubleref example

theories/examples/doubleref.v
@@ -3,20 +3,6 @@ From iris.base_logic.lib Require Import invariants.
 From iris.heap_lang Require Import notation proofmode lib.par lib.spin_lock.
 From iris.algebra Require Import agree frac csum excl.
 
-Definition prog (prize : loc) (n m : nat) : expr :=
-  let: "a" := ref #n in
-  let: "b" := ref #m in
-  (
-    if: !"a" ≤ !"b"
-    then FAA #prize #1
-    else Skip
-  ) ||| (
-    if: !"b" < !"a"
-    then FAA #prize #1
-    else Skip
-  );;
-  #().
-
 Definition prog_simpler (prize : loc) (l : loc) : expr :=
   (
     if: !#l = #0
@@ -32,62 +18,10 @@ Definition prog_simpler (prize : loc) (l : loc) : expr :=
 Section Proofs.
   Context `{heapG Σ}.
 
-  Lemma wp_prog prize n m:
-    ({{{ prize ↦ #0 }}} prog prize n m {{{ RET #(); prize ↦ #1 }}})%I.
-  Proof.
-    iIntros (Φ) "!> Hprize HΦ".
-    rewrite /prog.
-    wp_alloc a as "Ha". wp_pures.
-    wp_alloc b as "Hb". wp_pures.
-    iCombine "Ha Hb" as "Hab".
-    iMod (inv_alloc nroot with "Hab") as "#Hinv".
-    wp_pures.
-    wp_bind (par _ _)%E.
-    wp_apply (wp_par (λ _, True%I) (λ _, True%I)).
-    - (* Thread 1 *)
-      wp_bind (! _)%E.
-      iInv "Hinv" as ">[Ha Hb]" "Hclose".
-      wp_load.
-      iMod ("Hclose" with "[Ha Hb]").
-      { iModIntro. iFrame "Ha Hb". }
-      iModIntro.
-
-      wp_bind (! _)%E.
-      iInv "Hinv" as ">[Ha Hb]" "Hclose".
-      wp_load.
-      iMod ("Hclose" with "[Ha Hb]").
-      { iModIntro. iFrame "Ha Hb". }
-      iModIntro.
-
-      wp_pures. case_bool_decide; wp_pures.
-      + (* n ≤ m *)
-        admit.
-      + (* n > m *)
-        admit.
-
-    - (* Thread 2 *)
-      wp_bind (! _)%E.
-      iInv "Hinv" as ">[Ha Hb]" "Hclose".
-      wp_load.
-      iMod ("Hclose" with "[Ha Hb]").
-      { iModIntro. iFrame "Ha Hb". }
-      iModIntro.
-
-      wp_bind (! _)%E.
-      iInv "Hinv" as ">[Ha Hb]" "Hclose".
-      wp_load.
-      iMod ("Hclose" with "[Ha Hb]").
-      { iModIntro. iFrame "Ha Hb". }
-      iModIntro.
-      wp_pures. case_bool_decide; wp_pures.
-      + (* n > m *)
-        admit.
-      + (* n ≤ m *)
-        admit.
-  Admitted.
-
   Lemma wp_prog_simpler (prize l : loc) (k : nat):
-    ({{{ prize ↦ #0 ∗ l ↦ #k }}} prog_simpler prize l {{{ RET #(); prize ↦ #1 ∗ l ↦ #k }}})%I.
+    ({{{ prize ↦ #0 ∗ l ↦ #k }}}
+       prog_simpler prize l
+     {{{ RET #(); prize ↦ #1 ∗ l ↦ #k }}})%I.
   Proof.
     iIntros (Φ) "!> [Hprize Hl] HΦ".
     iMod (inv_alloc nroot with "Hl") as "#Hinv".
@@ -107,6 +41,7 @@ Section Proofs.
         admit.
       + (* n ≠ 0 *)
         done.
+
     - (* Thread 2*)
       wp_bind (! _)%E.
       iInv "Hinv" as ">Hl" "Hclose".
@@ -115,9 +50,9 @@ Section Proofs.
       iModIntro.
 
       wp_pures. case_bool_decide; wp_pures.
-      + (* n ≠ 0 *)
-        done.
       + (* n = 0 *)
+        done.
+      + (* n ≠ 0 *)
         admit.
 
     - iIntros (? ?) "[_ _]". iModIntro.
